\documentclass[twoside, a4paperpt, fleqn]{extarticle}
\usepackage{style}
\begin{document}
    \section*{Производные}
    \begin{multicols}{2}
        \begin{itemize}
            \item $\left(x^{n}\right)^{\prime}=n x^{n-1}$
            \item $\left(a^{x}\right)^{\prime}=a^{x} \cdot \ln a$
            \item $\left(e^{x}\right)^{\prime}=e^{x}$
            \item $\left(\log _{a} u\right)^{\prime}=\cfrac{u^{\prime}}{u \ln a}, \quad(\ln u)^{\prime}=\cfrac{u^{\prime}}{u}$
            \item $(\sin x)^{\prime}=\cos x, \quad(\cos x)^{\prime}=-\sin x$
            \item $(\sqrt{u})^{\prime}=\cfrac{u^{\prime}}{2 \sqrt{u}}$
            \item $(\operatorname{tgu})^{\prime}=\cfrac{u^{\prime}}{\cos ^{2} u}, \quad(c t g x)^{\prime}=-\cfrac{u^{\prime}}{\sin ^{2} u}$
            \item $(\arcsin x)^{\prime}=\cfrac{1}{\sqrt{1-x^{2}}}$
            \item $(\arccos x)^{\prime}=-\cfrac{1}{\sqrt{1-x}}$
            \item $(\operatorname{arctg} x)^{\prime}=\cfrac{1}{1+x^{2}}$
            \item $(\operatorname{arcctg} x)^{\prime}=-\cfrac{1}{1+x^{2}}$
            \item $(\operatorname{sh} x)^{\prime}=\operatorname{ch} x$
            \item $(\operatorname{ch} x)^{\prime}=\operatorname{sh} x$
            \item $(t h x)^{\prime}=\cfrac{1}{c h^{2} x}$
            \item $(\text { cth } x)^{\prime}=-\cfrac{1}{\operatorname{sh}^{2} x}$
            \item $\left(x^{x}\right)^{\prime}=x^{x} \cdot(1+\ln x)$
            \item $\left(\ln \left(x+\sqrt{1+x^{2}}\right)\right)^{\prime}=\cfrac{1}{\sqrt{1+x^{2}}}$
            \item $\left(\cfrac{1}{2} \ln \left(\cfrac{1+x}{1-x}\right)\right)^{\prime}=\cfrac{1}{1-x^{2}}$
            \item $(1 / x)^{(n)}=\cfrac{(-1)^{n} \cdot n !}{x^{n+1}}$
            \item $\left(a^{x}\right)^{(n)}=a^{x} \cdot \ln ^{n} x$
            \item $(\sin x)^{(n)}=\sin \left(x+\cfrac{\pi n}{2}\right)$
            \item $(\cos x)^{(n)}=\cos \left(x+\cfrac{\pi n}{2}\right)$
            \item $(\ln x)^{(n)}=\cfrac{(-1)^{(n-1)} \cdot(n-1) !}{x^{n}}$
        \end{itemize}
    \end{multicols}
    \begin{itemize}
        \item $\left(u^{v}\right)^{\prime}=v \cdot u^{v-1} \cdot u^{\prime}+u^{v} \cdot \ln u \cdot v^{\prime}$ - $\left(\sqrt{1+x^{2}}\right)^{\prime}=\cfrac{x}{\sqrt{x^{2}+1}}$
    \end{itemize}
\end{document}